\documentclass{mumie.element.exercise}
%$Id$
\begin{metainfo}
  \name{
    \lang{de}{Ü05: Grenzwerte}
    \lang{en}{}
  }
  \begin{description} 
 This work is licensed under the Creative Commons License Attribution 4.0 International (CC-BY 4.0)   
 https://creativecommons.org/licenses/by/4.0/legalcode 

    \lang{de}{Hier die Beschreibung}
    \lang{en}{}
  \end{description}
  \begin{components}
  \end{components}
  \begin{links}
  \end{links}
  \creategeneric
\end{metainfo}
\begin{content}
\title{
\lang{de}{Ü05: Grenzwerte}
}
\begin{block}[annotation]
  Im Ticket-System: \href{http://team.mumie.net/issues/9989}{Ticket 9989}
\end{block}
 
\lang{de}{Bestimmen Sie folgende Grenzwerte}
\begin{enumerate}
\item
\begin{table}[\class{items}]
  \nowrap{a) 
  $\displaystyle \lim_{x\to -1}\frac{x+1}{x-1}$} & 
  \nowrap{b) 
  $\displaystyle \lim_{x\to -1}\frac{x^2+4x+3}{x+1}$} 
\end{table}
\item
\begin{table}[\class{items}]
  \nowrap{a) 
  $\displaystyle \lim_{x\to \infty}\frac{3^x}{x^3}$} &
  \nowrap{b) 
  $\displaystyle \lim_{x\to \infty}\frac{x^2+x}{4^x}$} &
  \nowrap{c) 
  $\displaystyle \lim_{x\to \infty}3^{-x}x^5$}\\
   \nowrap{d) 
  $\displaystyle \lim_{x\to -\infty}4^x\cdot x^3$} &
  \nowrap{e) 
  $\displaystyle \lim_{x\to -\infty}\left(\frac{1}{2}\right)^x\cdot x^2$} &
  \nowrap{f) 
  $\displaystyle \lim_{x\to -\infty}\frac{2^x}{x}$}\\
   \nowrap{g) 
  $\displaystyle \lim_{x\to \infty}\frac{x^2+3x-1}{x+2}$} &
  \nowrap{h) 
  $\displaystyle \lim_{x\to \infty}\frac{x-1}{2x^2+x+1}$} &
  \nowrap{i) 
  $\displaystyle \lim_{x\to \infty}\frac{3x+4}{4x-1}$}\\
   \nowrap{j) 
  $\displaystyle \lim_{x\to \infty}\frac{(2x-1)^2}{x^2+1}$} &
  \nowrap{k) 
  $\displaystyle \lim_{x\to \infty}\frac{x^3}{1-x^2}$} &
  \nowrap{l) 
  $\displaystyle \lim_{x\to -\infty}\frac{x^3}{1-x^2}$}\\
   \nowrap{m) 
  $\displaystyle \lim_{x\to \infty}\frac{x}{\log_2 x}$} &
  \nowrap{n) 
  $\displaystyle \lim_{x\to \infty}\frac{(\ln x)^2}{x}$} &
  \nowrap{o) 
  $\displaystyle \lim_{x\to \downarrow 0}x^2\cdot \log_4 x$}\\
   \nowrap{p) 
  $\displaystyle \lim_{x\to \downarrow 0}\frac{x}{\ln x}$} &
  \nowrap{q) 
  $\displaystyle \lim_{x\to \downarrow 0}\frac{2^{\frac{1}{x}}}{x}$} &
  \nowrap{r) 
  $\displaystyle \lim_{x\to \uparrow 0}\frac{2^{\frac{1}{x}}}{x}$}\\
\end{table}
\end{enumerate}



\begin{tabs*}[\initialtab{0}\class{exercise}]

  \tab{
  \lang{de}{Antworten }}
  \begin{enumerate}
  \item 
  \begin{table}[\class{items}]
  \nowrap{a) 
  $\displaystyle \lim_{x\to -1}\frac{x+1}{x-1}=0$} & 
  \nowrap{b) 
  $\displaystyle \lim_{x\to -1}\frac{x^2+4x+3}{x+1}=2$} 
\end{table}
  \item 
  \begin{table}[\class{items}]
  \nowrap{a) 
  $\displaystyle \lim_{x\to \infty}\frac{3^x}{x^3}=\infty$} &
  \nowrap{b) 
  $\displaystyle \lim_{x\to \infty}\frac{x^2+x}{4^x}=0$} &
  \nowrap{c) 
  $\displaystyle \lim_{x\to \infty}3^{-x}x^5=0$}\\
   \nowrap{d) 
  $\displaystyle \lim_{x\to -\infty}4^x\cdot x^3=0$} &
  \nowrap{e) 
  $\displaystyle \lim_{x\to -\infty}\left(\frac{1}{2}\right)^x\cdot x^2=\infty$} &
  \nowrap{f) 
  $\displaystyle \lim_{x\to -\infty}\frac{2^x}{x}=0$}\\
   \nowrap{g) 
  $\displaystyle \lim_{x\to \infty}\frac{x^3+3x-1}{x+2}=\infty$} &
  \nowrap{h) 
  $\displaystyle \lim_{x\to \infty}\frac{x-1}{2x^2+x+1}=0$} &
  \nowrap{i) 
  $\displaystyle \lim_{x\to \infty}\frac{3x+4}{4x-1}=\frac{3}{4}$}\\
   \nowrap{j) 
  $\displaystyle \lim_{x\to \infty}\frac{(2x-1)^2}{x^2+1}=4$} &
  \nowrap{k) 
  $\displaystyle \lim_{x\to \infty}\frac{x^3}{1-x^2}=-\infty$} &
  \nowrap{l) 
  $\displaystyle \lim_{x\to -\infty}\frac{x^3}{1-x^2}=\infty$}\\
   \nowrap{m) 
  $\displaystyle \lim_{x\to \infty}\frac{x}{\log_2 x}=\infty$} &
  \nowrap{n) 
  $\displaystyle \lim_{x\to \infty}\frac{(\ln x)^2}{x}=0$} &
  \nowrap{o) 
  $\displaystyle \lim_{x\to \downarrow 0}x^2\cdot \log_4 x=0$}\\
   \nowrap{p) 
  $\displaystyle \lim_{x\to \downarrow 0}\frac{x}{\ln x}=0$} &
  \nowrap{q) 
  $\displaystyle \lim_{x\to \downarrow 0}\frac{2^{\frac{1}{x}}}{x}=\infty$} &
  \nowrap{r) 
  $\displaystyle \lim_{x\to \uparrow 0}\frac{2^{\frac{1}{x}}}{x}=0$}\\
\end{table}
  
\end{enumerate}
  
 
    \tab{
  \lang{de}{Lösung 1)}}
a) Es gilt
    \[
     \lim_{x\to -1}\frac{x+1}{x-1}\underset{\text{GWS}}{=}\frac{-1+1}{-1-1}=0.
    \]  
b) Es gilt
    \[
     \lim_{x\to -1}\frac{x^2+4x+3}{x+1}=\lim_{x\to -1}\frac{(x+1)(x+3)}{x+1}=\lim_{x\to -1}(x+3)=2.
    \]
  
       \tab{\lang{de}{Lösungsvideo 2)}}	
    \youtubevideo[500][300]{c42EVCzmY2Q}\\
  
  
\end{tabs*}

\end{content}