\documentclass{mumie.element.exercise}
%$Id$
\begin{metainfo}
  \name{
    \lang{de}{Ü03: Ableitung der Umkehrfunktion}
    \lang{en}{Exercise 3: derivative of inverse functions}
  }
  \begin{description} 
 This work is licensed under the Creative Commons License Attribution 4.0 International (CC-BY 4.0)   
 https://creativecommons.org/licenses/by/4.0/legalcode 

    \lang{de}{}
    \lang{en}{}
  \end{description}
  \begin{components}
  \end{components}
  \begin{links}
  \end{links}
  \creategeneric
\end{metainfo}
\begin{content}
\title{\lang{de}{Ü03: Ableitung der Umkehrfunktion}
    \lang{en}{Exercise 3: derivative of inverse functions}}


\begin{block}[annotation]
	Im Ticket-System: \href{https://team.mumie.net/issues/24021}{Ticket 24021}
\end{block}
\usepackage{mumie.ombplus}



\begin{block}[annotation]
Kopie: hm4mint/T301_Differenzierbarkeit/exercise 6

Im Ticket-System: \href{http://team.mumie.net/issues/10279}{Ticket 10279}
\end{block}

%######################################################FRAGE_TEXT
\lang{de}{ Gegeben ist die Funktion
\[ f:(0,\infty)\to\R,x\mapsto xe^x. \]
Bestimmen Sie die Ableitung der Umkehrfunktion von $f$ an der Stelle $e$.
 }

 \lang{en}{ Let $f$ be the function
\[ f:(0,\infty)\to\R,x\mapsto xe^x. \]
Find the derivative of the inverse of $f$ at the point $e$.
 }

%##################################################ANTWORTEN_TEXT
\begin{tabs*}[\initialtab{0}\class{exercise}]


  
  %++++++++++++++++++++++++++++++++++++++++++START_TAB_X
  \tab{\lang{de}{    Lösung)    }  \lang{en}{Solution}}
  \begin{incremental}[\initialsteps{1}]
  
  	 %----------------------------------START_STEP_X
    \step 
    \lang{de}{      Nach der Formel für die Ableitung der Umkehrfunktion ist
\[  (f^{-1})'(e)=\frac{1}{f'(f^{-1}(e))}. \]
 $f^{-1}(e)$ ist die Stelle $x_0$, für die $f(x_0)=e$ gilt. Wie leicht zu sehen ist,
 ist $f(1)=1\cdot e^1=e$, also $f^{-1}(e)=1$.
 
Da $f'(x)=(1+x)e^x$ ist, gilt also
\[  (f^{-1})'(e)=\frac{1}{f'(f^{-1}(e))}=\frac{1}{f'(1)}=\frac{1}{2e}. \]
 }
 \lang{en}{  According to the formula for the derivative of an inverse function,
\[  (f^{-1})'(e)=\frac{1}{f'(f^{-1}(e))}. \]
 $f^{-1}(e)$ is the point $x_0$ at which $f(x_0)=e$. It is easy to see that
 $f(1)=1\cdot e^1=e$ and therefore $f^{-1}(e)=1$.
 
Since $f'(x)=(1+x)e^x$, we find
\[  (f^{-1})'(e)=\frac{1}{f'(f^{-1}(e))}=\frac{1}{f'(1)}=\frac{1}{2e}. \]
 }
  	 %------------------------------------END_STEP_X
 
  \end{incremental}
  %++++++++++++++++++++++++++++++++++++++++++++END_TAB_X


%#############################################################ENDE
\end{tabs*}
\end{content}